src/xor/tseitin_xor.lean
@@ -24,18 +24,20 @@ variables {V : Type u} [inhabited V] [decidable_eq V]
 open literal
 open clause
 open cnf
-open nxor
+open Xor
 open encoding
+open gensym
 
+open nat
 open list
 open assignment
 open function
 
 namespace tseitin_xor
 
-lemma disjoint_fresh_of_disjoint {x : nxor V} {g : gensym V} {k : nat} (hk : k ≥ 3) :
+lemma disjoint_fresh_of_disjoint {x : Xor V} {g : gensym V} {k : nat} (hk : k ≥ 3) :
   disjoint g.stock x.vars → 
-  disjoint g.fresh.2.stock (nxor.vars ((Pos g.fresh.1) :: (x.drop (k - 1)))) :=
+  disjoint g.fresh.2.stock (Xor.vars ((Pos g.fresh.1) :: (x.drop (k - 1)))) :=
 begin
   intro h,
   apply set.disjoint_right.mpr,
@@ -43,14 +45,14 @@ begin
   simp [vars, clause.vars] at hv,
   rcases hv with rfl | hv,
   { rw var,
-    exact gensym.fresh_not_mem_fresh_stock g },
+    exact fresh_not_mem_fresh_stock g },
   { intro hcon,
-    have := clause.vars_subset_of_subset (drop_subset (k - 1) x),
     rw set.disjoint_right at h,
-    exact absurd ((gensym.fresh_stock_subset g) hcon) (h (this hv)) }
+    have := vars_subset_of_subset (drop_subset (k - 1) x),
+    exact absurd ((fresh_stock_subset g) hcon) (h (this hv)) }
 end
 
-lemma drop_len_lt {k : nat} {x : nxor V} (l : literal V) :
+lemma drop_len_lt {k : nat} {x : Xor V} (l : literal V) :
   k ≥ 3 → length x > k → length (l :: (x.drop (k - 1))) < length x :=
 begin
   intros hk hx,
@@ -60,11 +62,11 @@ begin
   rw [add_comm k x₂.length, nat.add_sub_assoc (nat.sub_le k 1),
       nat.sub_sub_self (nat.le_of_add_le_right hk), add_assoc],
   apply add_lt_add_left,
-  exact nat.succ_le_iff.mp hk,
+  exact succ_le_iff.mp hk,
 end
 
 -- Note: x and g can be made implicit args
-def linear_xor {k : nat} (hk : k ≥ 3) : Π (x : nxor V), Π (g : gensym V),
+def linear_xor {k : nat} (hk : k ≥ 3) : Π (x : Xor V), Π (g : gensym V),
   (disjoint g.stock x.vars) → cnf V
 | x g hdis := if h : length x ≤ k then direct_xor x else
                 have length ((Pos g.fresh.1) :: (x.drop (k - 1))) < length x,
@@ -77,12 +79,12 @@ using_well_founded {
   dec_tac := tactic.assumption
 }
 
-lemma linear_base_case {k : nat} (hk : k ≥ 3) {x : nxor V} {g : gensym V}
+lemma linear_base_case {k : nat} (hk : k ≥ 3) {x : Xor V} {g : gensym V}
   (hdis : disjoint g.stock x.vars) : 
   length x ≤ k → linear_xor hk x g hdis = direct_xor x :=
 assume h, by { rw linear_xor, simp only [h, if_true] }
 
-theorem mem_linear_xor_vars_of_mem_vars {k : nat} (hk : k ≥ 3) {x : nxor V} {g : gensym V}
+theorem mem_linear_xor_vars_of_mem_vars {k : nat} (hk : k ≥ 3) {x : Xor V} {g : gensym V}
   (hdis : disjoint g.stock x.vars) {v : V} :
   v ∈ x.vars → v ∈ (linear_xor hk x g hdis).vars :=
 begin
@@ -101,11 +103,12 @@ begin
     { rw not_le at hx,
       have h₁ := drop_len_lt (Pos g.fresh.1) hk hx,
       have h₂ := disjoint_fresh_of_disjoint hk hdis,
-      have := ih _ h₁ h₂ (clause.mem_vars_cons_of_mem_vars _ h),
+      have := ih _ h₁ h₂ (mem_vars_cons_of_mem_vars _ h),
       exact finset.mem_union_right _ this } }
 end
 
-theorem not_mem_linear_xor_vars_of_not_mem_vars_of_not_mem_stock {k : nat} (hk : k ≥ 3) {x : nxor V} {g : gensym V}
+theorem not_mem_linear_xor_vars_of_not_mem_vars_of_not_mem_stock 
+  {k : nat} (hk : k ≥ 3) {x : Xor V} {g : gensym V}
   (hdis : disjoint g.stock x.vars) {v : V} :
   v ∉ x.vars → v ∉ g.stock → v ∉ (linear_xor hk x g hdis).vars :=
 begin
@@ -113,39 +116,39 @@ begin
   by_cases hx : length x ≤ k,
   { rw [linear_base_case hk hdis hx, vars_direct_xor x], tautology },
   { intros hvars hg,
+    rw vars at hvars,
     rw linear_xor,
     simp [hx],
     rw cnf.vars_append,
     apply finset.not_mem_union.mpr,
-    rw vars at hvars,
     split,
     { rw [vars_direct_xor, vars, clause.vars_append],
       apply finset.not_mem_union.mpr,
       split,
       { intro hcon,
-        have := (clause.vars_subset_of_subset (take_subset (k - 1) x)),
+        have := (vars_subset_of_subset (take_subset (k - 1) x)),
         exact absurd (this hcon) hvars },
       { simp [var],
         intro hcon,
         rw hcon at hg,
-        exact absurd (gensym.fresh_mem_stock g) hg } },
+        exact absurd (fresh_mem_stock g) hg } },
     { have h₁ := drop_len_lt (Pos g.fresh.1) hk (not_le.mp hx),
       have h₂ := disjoint_fresh_of_disjoint hk hdis,
       have h₃ : v ∉ vars (Pos g.fresh.1 :: drop (k - 1) x),
       { simp [vars, clause.vars, var],
         rintros (rfl | h),
-        { exact hg (gensym.fresh_mem_stock g) },
+        { exact hg (fresh_mem_stock g) },
         { exact hvars (vars_subset_of_subset (drop_subset (k - 1) x) h) } },
       have h₄ : v ∉ g.fresh.2.stock,
       { intro hcon,
-        exact hg ((gensym.fresh_stock_subset g) hcon) },
+        exact hg ((fresh_stock_subset g) hcon) },
       exact ih _ h₁ h₂ h₃ h₄ } }
 end
 
 -- A slightly stronger statement
-lemma linear_forward {k : nat} (hk : k ≥ 3) {x : nxor V} {g : gensym V}
-  (hdis : disjoint g.stock x.vars) {α : assignment V} :
-  cnf.eval α (linear_xor hk x g hdis) = tt → cnf.eval α (direct_xor x) = tt :=
+lemma linear_forward {k : nat} (hk : k ≥ 3) {x : Xor V} {g : gensym V}
+  (hdis : disjoint g.stock x.vars) {τ : assignment V} :
+  cnf.eval τ (linear_xor hk x g hdis) = tt → cnf.eval τ (direct_xor x) = tt :=
 begin
   induction x using strong_induction_on_lists with x ih generalizing g,
   by_cases hx : length x ≤ k,
@@ -154,123 +157,144 @@ begin
     rw linear_xor at h,
     simp [hx, cnf.eval_append] at h,
     rcases h with ⟨hdir, hrec⟩,
-    rw not_le at hx,
-    have h₁ := drop_len_lt (Pos g.fresh.1) hk hx,
+    have h₁ := drop_len_lt (Pos g.fresh.1) hk (not_le.mp hx),
     have h₂ := disjoint_fresh_of_disjoint hk hdis,
     have ihred := ih _ h₁ h₂ hrec,
-    rw [eval_direct_xor_eq_eval_nxor, eval_eq_bodd_count_tt] at ihred,
-    rw [eval_direct_xor_eq_eval_nxor, eval_eq_bodd_count_tt] at hdir,
-    rw [eval_direct_xor_eq_eval_nxor, eval_eq_bodd_count_tt],
-    have := take_append_drop (k - 1) x,
-    have := congr_arg ((clause.count_tt α)) this,
-    have := congr_arg (nat.bodd) this,
-    cases hnew : (α g.fresh.1),
-    { simp [count_tt_cons, hnew, literal.eval] at ihred,
-      simp [count_tt_append, hnew, literal.eval] at hdir,
-      rw [count_tt_append, nat.bodd_add, hdir, ihred, ff_bxor] at this,
-      exact this.symm },
-    { simp [count_tt_cons, hnew, literal.eval] at ihred,
-      simp [count_tt_append, hnew, literal.eval] at hdir,
-      rw [count_tt_append, nat.bodd_add, hdir, ihred, bxor_ff] at this,
-      exact this.symm } }
+    rw [eval_direct_xor_eq_eval_Xor, eval_eq_bodd_count_tt] at ihred hdir |-,
+    have := congr_arg ((clause.count_tt τ)) (take_append_drop (k - 1) x).symm,
+    have := congr_arg bodd this,
+    cases hnew : (τ g.fresh.1),
+    { simp [count_tt_cons, count_tt_append, hnew, literal.eval] at ihred hdir,
+      rw [count_tt_append, bodd_add, hdir, ihred, ff_bxor] at this,
+      exact this },
+    { simp [count_tt_cons, count_tt_append, hnew, literal.eval] at ihred hdir,
+      rw [count_tt_append, bodd_add, hdir, ihred, bxor_ff] at this,
+      exact this } }
 end
 
-theorem linear_sequiv {k : nat} (hk : k ≥ 3) {x : nxor V} {g : gensym V}
+theorem linear_sequiv {k : nat} (hk : k ≥ 3) {x : Xor V} {g : gensym V}
   (hdis : disjoint g.stock x.vars) :
   sequiv (linear_xor hk x g hdis) (direct_xor x) x.vars :=
 begin
   induction x using strong_induction_on_lists with x ih generalizing g,
   by_cases hx : length x ≤ k,
   { rw linear_base_case hk hdis hx },
-  { intro τ,
-    split,
+  { intro τ, split,
     -- forward direction: linear -> direct
     { rintros ⟨σ, hl, hs⟩,
       use [σ, linear_forward hk hdis hl, hs] },
     -- reverse direction: direct -> linear
     { rintros ⟨σ, he, hs⟩,
 
-      rw [eval_direct_xor_eq_eval_nxor, eval_eq_bodd_count_tt] at he,
-      have htakedrop := take_append_drop (k - 1) x,
-      have hnotmem := set.disjoint_left.mp hdis (g.fresh_mem_stock),
-      rw [← htakedrop, count_tt_append, nat.bodd_add] at he, 
+      rw [eval_direct_xor_eq_eval_Xor, eval_eq_bodd_count_tt,
+        ← (take_append_drop (k - 1) x), count_tt_append, bodd_add] at he,
 
+      have hnotmem := set.disjoint_left.mp hdis (g.fresh_mem_stock),
       have h₁ := drop_len_lt (Pos g.fresh.1) hk (not_le.mp hx),
-      have h₂ := disjoint_fresh_of_disjoint hk hdis, 
+      have h₂ := disjoint_fresh_of_disjoint hk hdis,
+
+      have htakevars := vars_subset_of_subset (take_subset (k - 1) x),
+      have hdropvars := vars_subset_of_subset (drop_subset (k - 1) x),
 
       rw linear_xor,
       simp [hx, cnf.eval_append],
 
-      cases hc : nat.bodd (clause.count_tt σ (take (k - 1) x)),
-      { simp [hc] at he,
+      -- Case on the truth value of the last n - k + 1 variables
+      -- Note: the proof is symmetric, so any tightening-up can be done in both
+      cases hc : bodd (clause.count_tt σ (take (k - 1) x)),
+      { rw [hc, bool.bxor_ff_left] at he,
         rcases exists_eqod_and_eq_of_not_mem σ ff hnotmem with ⟨γ, heqod, hg⟩,
-        have : nat.bodd (clause.count_tt γ (Pos g.fresh.1 :: drop (k - 1) x)) = tt,
-        { simp only [count_tt_cons, literal.eval, hg, cond],
-          rw ← count_tt_eq_of_eqod (eqod_subset (vars_subset_of_subset (drop_subset (k - 1) x)) heqod),
-          exact he },
-        rw [← eval_eq_bodd_count_tt, ← eval_direct_xor_eq_eval_nxor] at this,
+        have : bodd (clause.count_tt γ (Pos g.fresh.1 :: drop (k - 1) x)) = tt,
+        { simp only [count_tt_cons, literal.eval, hg, cond,
+            ← count_tt_eq_of_eqod (eqod_subset hdropvars heqod), he] },
+        rw [← eval_eq_bodd_count_tt, ← eval_direct_xor_eq_eval_Xor] at this,
 
         -- Apply the induction hypothesis
         rcases (ih _ h₁ h₂ γ).mpr ⟨γ, this, eqod.refl _ _⟩ with ⟨γ₂, he₂, hg₂⟩,
-        have hg₂copy := hg₂,
-        rw [vars, clause.vars, var] at hg₂copy,
-        have := eqod_subset (finset.subset_union_right {g.fresh.1} (clause.vars (x.drop (k - 1)))) hg₂copy,
 
-        have bigeqod : eqod (assignment.ite (cnf.vars (linear_xor hk (Pos g.fresh.1 :: (x.drop (k - 1))) g.fresh.2 h₂)) γ₂ γ) γ (clause.vars x),
-        {
-          intros v hv,
+        have heqod₂ : eqod (assignment.ite (cnf.vars (linear_xor hk (Pos g.fresh.1 :: (x.drop (k - 1))) g.fresh.2 h₂)) γ₂ γ) γ (clause.vars x),
+        { intros v hv,
           by_cases hmem : v ∈ vars (x.drop (k - 1)),
           { rw vars at hmem,
-            have h₃ := clause.mem_vars_cons_of_mem_vars (Pos g.fresh.1) hmem,
-            have := mem_linear_xor_vars_of_mem_vars hk h₂ h₃,
-            rw ite_pos _ _ this,
-            rw hg₂ v h₃ },
-          {
-            have hdis₂ := set.disjoint_right.mp hdis hv,
+            have h₃ := mem_vars_cons_of_mem_vars (Pos g.fresh.1) hmem,
+            rw [ite_pos _ _ (mem_linear_xor_vars_of_mem_vars hk h₂ h₃), hg₂ v h₃] },
+          { have hdis₂ := set.disjoint_right.mp hdis hv,
             have hne : v ≠ g.fresh.1,
             { intro hcon,
-              rw hcon at hdis₂,
-              exact hdis₂ (gensym.fresh_mem_stock g) },
+              exact (hcon ▸ hdis₂) (fresh_mem_stock g) },
             have : v ∉ vars (Pos g.fresh.1 :: drop (k - 1) x),
             { simp [vars, clause.vars, var],
               rintros (hcon | hcon),
               { exact hne hcon },
               { rw vars at hmem, exact hmem hcon } },
-            have hdis₃ := gensym.fresh_stock_subset g,
             have hstock : v ∉ g.fresh.2.stock,
             { intro hcon,
-              exact hdis₂ (hdis₃ hcon) },
-            have := not_mem_linear_xor_vars_of_not_mem_vars_of_not_mem_stock hk h₂ this hstock,
-            rw ite_neg _ _ this } },
+              exact hdis₂ ((fresh_stock_subset g) hcon) },
+            rw ite_neg _ _ (not_mem_linear_xor_vars_of_not_mem_vars_of_not_mem_stock hk h₂ this hstock) } },
         
         use assignment.ite (cnf.vars (linear_xor hk (Pos g.fresh.1 :: (x.drop (k - 1))) g.fresh.2 h₂)) γ₂ γ,
-        
         split,
         { split,
-          { simp [eval_direct_xor_eq_eval_nxor, eval_eq_bodd_count_tt, 
-              count_tt_append, nat.bodd_add, literal.eval, hg],
+          { simp [eval_direct_xor_eq_eval_Xor, eval_eq_bodd_count_tt, 
+              count_tt_append, bodd_add, literal.eval, hg],
             have : g.fresh.1 ∈ vars (Pos g.fresh.1 :: (x.drop (k - 1))),
             { exact mem_vars_cons_self _ _ },
-            have := mem_linear_xor_vars_of_mem_vars hk h₂ this,
-            rw ite_pos _ _ this,
-            have := clause.mem_vars_cons_self (Pos g.fresh.1) (x.drop (k - 1)),
-            rw var at this,
-            rw ← (hg₂ g.fresh.1 this),
-            simp [hg],
-            have := eqod_subset (vars_subset_of_subset (take_subset (k - 1) x)) bigeqod,
-            rw count_tt_eq_of_eqod this,
-            rw ← count_tt_eq_of_eqod (eqod_subset (vars_subset_of_subset (take_subset (k - 1) x)) heqod),
-            exact hc },
-          { rw eval_eq_cnf_of_eqod (ite_eqod _ _ _),
-            exact he₂ } },
-        { exact eqod.trans (eqod.trans hs heqod) bigeqod.symm } },
-      { sorry, } } }
+            simp [ite_pos _ _ (mem_linear_xor_vars_of_mem_vars hk h₂ this), 
+              ← (hg₂ g.fresh.1 this), hg,
+              count_tt_eq_of_eqod (eqod_subset htakevars heqod₂),
+              ← count_tt_eq_of_eqod (eqod_subset htakevars heqod), hc] },
+          { exact he₂ ▸ eval_eq_cnf_of_eqod (ite_eqod _ _ _) } },
+        { exact eqod.trans (eqod.trans hs heqod) heqod₂.symm } },
+      { simp only [hc, bnot_eq_true_eq_eq_ff, tt_bxor] at he,
+        rcases exists_eqod_and_eq_of_not_mem σ tt hnotmem with ⟨γ, heqod, hg⟩,
+        have : bodd (clause.count_tt γ (Pos g.fresh.1 :: drop (k - 1) x)) = tt,
+        { simp only [count_tt_cons, literal.eval, hg, cond, 
+            ← count_tt_eq_of_eqod (eqod_subset hdropvars heqod), he, bodd_succ, 
+            bodd_add, bodd_zero, bool.bnot_false, bool.bxor_ff_right], },
+        rw [← eval_eq_bodd_count_tt, ← eval_direct_xor_eq_eval_Xor] at this,
+
+        -- Apply the induction hypothesis
+        rcases (ih _ h₁ h₂ γ).mpr ⟨γ, this, eqod.refl _ _⟩ with ⟨γ₂, he₂, hg₂⟩,
+
+        have heqod₂ : eqod (assignment.ite (cnf.vars (linear_xor hk (Pos g.fresh.1 :: (x.drop (k - 1))) g.fresh.2 h₂)) γ₂ γ) γ (clause.vars x),
+        { intros v hv,
+          by_cases hmem : v ∈ vars (x.drop (k - 1)),
+          { rw vars at hmem,
+            have h₃ := mem_vars_cons_of_mem_vars (Pos g.fresh.1) hmem,
+            rw [ite_pos _ _ (mem_linear_xor_vars_of_mem_vars hk h₂ h₃), hg₂ v h₃] },
+          { have hdis₂ := set.disjoint_right.mp hdis hv,
+            have hne : v ≠ g.fresh.1,
+            { intro hcon,
+              exact (hcon ▸ hdis₂) (fresh_mem_stock g) },
+            have : v ∉ vars (Pos g.fresh.1 :: drop (k - 1) x),
+            { simp [vars, clause.vars, var],
+              rintros (hcon | hcon),
+              { exact hne hcon },
+              { rw vars at hmem, exact hmem hcon } },
+            have hstock : v ∉ g.fresh.2.stock,
+            { intro hcon,
+              exact hdis₂ ((fresh_stock_subset g) hcon) },
+            rw ite_neg _ _ (not_mem_linear_xor_vars_of_not_mem_vars_of_not_mem_stock hk h₂ this hstock) } },
+        
+        use assignment.ite (cnf.vars (linear_xor hk (Pos g.fresh.1 :: (x.drop (k - 1))) g.fresh.2 h₂)) γ₂ γ,
+        split,
+        { split,
+          { simp [eval_direct_xor_eq_eval_Xor, eval_eq_bodd_count_tt, 
+              count_tt_append, bodd_add, literal.eval, hg],
+            have : g.fresh.1 ∈ vars (Pos g.fresh.1 :: (x.drop (k - 1))),
+            { exact mem_vars_cons_self _ _ },
+            simp [ite_pos _ _ (mem_linear_xor_vars_of_mem_vars hk h₂ this), 
+              ← (hg₂ g.fresh.1 this), hg,
+              count_tt_eq_of_eqod (eqod_subset htakevars heqod₂),
+              ← count_tt_eq_of_eqod (eqod_subset htakevars heqod), hc] },
+          { exact he₂ ▸ eval_eq_cnf_of_eqod (ite_eqod _ _ _) } },
+        { exact eqod.trans (eqod.trans hs heqod) heqod₂.symm } } } }
 end
 
 -- Note: The proofs here are symmetric with the linear encoding ones
 -- If an improvement is made to the above proofs, simplify here
 
-lemma drop_len_lt' {k : nat} {x : nxor V} (l : literal V) :
+lemma drop_len_lt' {k : nat} {x : Xor V} (l : literal V) :
   k ≥ 3 → length x > k → length (x.drop (k - 1) ++ [l]) < length x :=
 begin
   have : (drop (k - 1) x ++ [l]).length = (l :: drop (k - 1) x).length,
@@ -279,9 +303,9 @@ begin
   exact drop_len_lt l
 end
 
-lemma disjoint_fresh_of_disjoint' {x : nxor V} {g : gensym V} {k : nat} (hk : k ≥ 3) :
+lemma disjoint_fresh_of_disjoint' {x : Xor V} {g : gensym V} {k : nat} (hk : k ≥ 3) :
   disjoint g.stock x.vars → 
-  disjoint g.fresh.2.stock (nxor.vars (x.drop (k - 1) ++ [Pos g.fresh.1])) :=
+  disjoint g.fresh.2.stock (Xor.vars (x.drop (k - 1) ++ [Pos g.fresh.1])) :=
 begin
   intro h,
   apply set.disjoint_right.mpr,
@@ -289,15 +313,15 @@ begin
   simp [vars, clause.vars, clause.vars_append] at hv,
   rcases hv with rfl | hv,
   { rw var,
-    exact gensym.fresh_not_mem_fresh_stock g },
+    exact fresh_not_mem_fresh_stock g },
   { intro hcon,
-    have := clause.vars_subset_of_subset (drop_subset (k - 1) x),
     rw set.disjoint_right at h,
-    exact absurd ((gensym.fresh_stock_subset g) hcon) (h (this hv)) }
+    have := vars_subset_of_subset (drop_subset (k - 1) x),
+    exact absurd ((fresh_stock_subset g) hcon) (h (this hv)) }
 end
 
 -- Note: x and g can be made implicit args
-def pooled_xor {k : nat} (hk : k ≥ 3) : Π (x : nxor V), Π (g : gensym V),
+def pooled_xor {k : nat} (hk : k ≥ 3) : Π (x : Xor V), Π (g : gensym V),
   (disjoint g.stock x.vars) → cnf V
 | x g hdis := if h : length x ≤ k then direct_xor x else
                 have length (x.drop (k - 1) ++ [Pos g.fresh.1]) < length x,
@@ -310,12 +334,12 @@ using_well_founded {
   dec_tac := tactic.assumption
 }
 
-lemma pooled_base_case {k : nat} (hk : k ≥ 3) {x : nxor V} {g : gensym V}
+lemma pooled_base_case {k : nat} (hk : k ≥ 3) {x : Xor V} {g : gensym V}
   (hdis : disjoint g.stock x.vars) : 
   length x ≤ k → pooled_xor hk x g hdis = direct_xor x :=
 assume h, by { rw pooled_xor, simp only [h, if_true] }
 
-theorem mem_pooled_xor_vars_of_mem_vars {k : nat} (hk : k ≥ 3) {x : nxor V} {g : gensym V}
+theorem mem_pooled_xor_vars_of_mem_vars {k : nat} (hk : k ≥ 3) {x : Xor V} {g : gensym V}
   (hdis : disjoint g.stock x.vars) {v : V} :
   v ∈ x.vars → v ∈ (pooled_xor hk x g hdis).vars :=
 begin
@@ -341,7 +365,8 @@ begin
       exact finset.mem_union_right _ this } }
 end
 
-theorem not_mem_pooled_xor_vars_of_not_mem_vars_of_not_mem_stock {k : nat} (hk : k ≥ 3) {x : nxor V} {g : gensym V}
+theorem not_mem_pooled_xor_vars_of_not_mem_vars_of_not_mem_stock {k : nat} 
+  (hk : k ≥ 3) {x : Xor V} {g : gensym V}
   (hdis : disjoint g.stock x.vars) {v : V} :
   v ∉ x.vars → v ∉ g.stock → v ∉ (pooled_xor hk x g hdis).vars :=
 begin
@@ -349,33 +374,182 @@ begin
   by_cases hx : length x ≤ k,
   { rw [pooled_base_case hk hdis hx, vars_direct_xor x], tautology },
   { intros hvars hg,
+    rw vars at hvars,
     rw pooled_xor,
     simp [hx],
     rw cnf.vars_append,
     apply finset.not_mem_union.mpr,
-    rw vars at hvars,
     split,
     { rw [vars_direct_xor, vars, clause.vars_append],
       apply finset.not_mem_union.mpr,
       split,
       { intro hcon,
-        have := (clause.vars_subset_of_subset (take_subset (k - 1) x)),
+        have := (vars_subset_of_subset (take_subset (k - 1) x)),
         exact absurd (this hcon) hvars },
       { simp [var],
         intro hcon,
         rw hcon at hg,
-        exact absurd (gensym.fresh_mem_stock g) hg } },
+        exact absurd (fresh_mem_stock g) hg } },
     { have h₁ := drop_len_lt' (Pos g.fresh.1) hk (not_le.mp hx),
       have h₂ := disjoint_fresh_of_disjoint' hk hdis,
       have h₃ : v ∉ vars (drop (k - 1) x ++ [Pos g.fresh.1]),
       { simp [vars, clause.vars, var, clause.vars_append],
         rintros (h | rfl),
         { exact hvars (vars_subset_of_subset (drop_subset (k - 1) x) h) },
-        { exact hg (gensym.fresh_mem_stock g) } },
+        { exact hg (fresh_mem_stock g) } },
       have h₄ : v ∉ g.fresh.2.stock,
       { intro hcon,
-        exact hg ((gensym.fresh_stock_subset g) hcon) },
+        exact hg ((fresh_stock_subset g) hcon) },
       exact ih _ h₁ h₂ h₃ h₄ } }
+end
+
+lemma pooled_forward {k : nat} (hk : k ≥ 3) {x : Xor V} {g : gensym V}
+  (hdis : disjoint g.stock x.vars) {τ : assignment V} :
+  cnf.eval τ (pooled_xor hk x g hdis) = tt → cnf.eval τ (direct_xor x) = tt :=
+begin
+  induction x using strong_induction_on_lists with x ih generalizing g,
+  by_cases hx : length x ≤ k,
+  { rw pooled_base_case hk hdis hx, exact id },
+  { intro h,
+    rw pooled_xor at h,
+    simp [hx, cnf.eval_append] at h,
+    rcases h with ⟨hdir, hrec⟩,
+    have h₁ := drop_len_lt' (Pos g.fresh.1) hk (not_le.mp hx),
+    have h₂ := disjoint_fresh_of_disjoint' hk hdis,
+    have ihred := ih _ h₁ h₂ hrec,
+    rw [eval_direct_xor_eq_eval_Xor, eval_eq_bodd_count_tt] at ihred hdir |-,
+    have := congr_arg ((clause.count_tt τ)) (take_append_drop (k - 1) x).symm,
+    have := congr_arg bodd this,
+    cases hnew : (τ g.fresh.1),
+    { simp [count_tt_cons, count_tt_append, hnew, literal.eval] at ihred hdir,
+      rw [count_tt_append, bodd_add, hdir, ihred, ff_bxor] at this,
+      exact this },
+    { simp [count_tt_cons, count_tt_append, hnew, literal.eval] at ihred hdir,
+      rw [count_tt_append, bodd_add, hdir, ihred, bxor_ff] at this,
+      exact this } }
+end
+
+theorem pooled_sequiv {k : nat} (hk : k ≥ 3) {x : Xor V} {g : gensym V}
+  (hdis : disjoint g.stock x.vars) :
+  sequiv (pooled_xor hk x g hdis) (direct_xor x) x.vars :=
+begin
+  induction x using strong_induction_on_lists with x ih generalizing g,
+  by_cases hx : length x ≤ k,
+  { rw pooled_base_case hk hdis hx },
+  { intro τ, split,
+    -- forward direction: pooled -> direct
+    { rintros ⟨σ, hl, hs⟩,
+      use [σ, pooled_forward hk hdis hl, hs] },
+    -- reverse direction: direct -> pooled 
+    { rintros ⟨σ, he, hs⟩,
+
+      rw [eval_direct_xor_eq_eval_Xor, eval_eq_bodd_count_tt,
+        ← (take_append_drop (k - 1) x), count_tt_append, bodd_add] at he,
+
+      have hnotmem := set.disjoint_left.mp hdis (g.fresh_mem_stock),
+      have h₁ := drop_len_lt' (Pos g.fresh.1) hk (not_le.mp hx),
+      have h₂ := disjoint_fresh_of_disjoint' hk hdis,
+
+      have htakevars := vars_subset_of_subset (take_subset (k - 1) x),
+      have hdropvars := vars_subset_of_subset (drop_subset (k - 1) x),
+
+      rw pooled_xor,
+      simp [hx, cnf.eval_append],
+
+      -- Case on the truth value of the last n - k + 1 variables
+      -- Note: the proof is symmetric, so any tightening-up can be done in both
+      cases hc : bodd (clause.count_tt σ (take (k - 1) x)),
+      { rw [hc, bool.bxor_ff_left] at he,
+        rcases exists_eqod_and_eq_of_not_mem σ ff hnotmem with ⟨γ, heqod, hg⟩,
+        have : bodd (clause.count_tt γ (drop (k - 1) x ++ [Pos g.fresh.1])) = tt,
+        { simp [count_tt_append, literal.eval, hg, cond,
+            ← count_tt_eq_of_eqod (eqod_subset hdropvars heqod), he] },
+        rw [← eval_eq_bodd_count_tt, ← eval_direct_xor_eq_eval_Xor] at this,
+
+        -- Apply the induction hypothesis
+        rcases (ih _ h₁ h₂ γ).mpr ⟨γ, this, eqod.refl _ _⟩ with ⟨γ₂, he₂, hg₂⟩,
+
+        have heqod₂ : eqod (assignment.ite (cnf.vars (pooled_xor hk (x.drop (k - 1) ++ [Pos g.fresh.1]) g.fresh.2 h₂)) γ₂ γ) γ (clause.vars x),
+        { intros v hv,
+          by_cases hmem : v ∈ vars (x.drop (k - 1)),
+          { rw vars at hmem,
+            have h₃ : v ∈ vars (drop (k - 1) x ++ [Pos g.fresh.1]),
+            { rw [vars, clause.vars_append],
+              exact finset.mem_union_left _ hmem },
+            rw [ite_pos _ _ (mem_pooled_xor_vars_of_mem_vars hk h₂ h₃), hg₂ v h₃] },
+          { have hdis₂ := set.disjoint_right.mp hdis hv,
+            have hne : v ≠ g.fresh.1,
+            { intro hcon,
+              exact (hcon ▸ hdis₂) (fresh_mem_stock g) },
+            have : v ∉ vars (drop (k - 1) x ++ [Pos g.fresh.1]),
+            { simp [vars, clause.vars, var, clause.vars_append],
+              rintros (hcon | hcon),
+              { rw vars at hmem, exact hmem hcon },
+              { exact hne hcon } },
+            have hstock : v ∉ g.fresh.2.stock,
+            { intro hcon,
+              exact hdis₂ ((fresh_stock_subset g) hcon) },
+            rw ite_neg _ _ (not_mem_pooled_xor_vars_of_not_mem_vars_of_not_mem_stock hk h₂ this hstock) } },
+        
+        use assignment.ite (cnf.vars (pooled_xor hk (drop (k - 1) x ++ [Pos g.fresh.1]) g.fresh.2 h₂)) γ₂ γ,
+        split,
+        { split,
+          { simp [eval_direct_xor_eq_eval_Xor, eval_eq_bodd_count_tt, 
+              count_tt_append, bodd_add, literal.eval, hg],
+            have : g.fresh.1 ∈ vars (drop (k - 1) x ++ [Pos g.fresh.1]),
+            { simp [vars, clause.vars_append, var] },
+            simp [ite_pos _ _ (mem_pooled_xor_vars_of_mem_vars hk h₂ this), 
+              ← (hg₂ g.fresh.1 this), hg,
+              count_tt_eq_of_eqod (eqod_subset htakevars heqod₂),
+              ← count_tt_eq_of_eqod (eqod_subset htakevars heqod), hc] },
+          { exact he₂ ▸ eval_eq_cnf_of_eqod (ite_eqod _ _ _) } },
+        { exact eqod.trans (eqod.trans hs heqod) heqod₂.symm } },
+      { simp only [hc, bnot_eq_true_eq_eq_ff, tt_bxor] at he,
+        rcases exists_eqod_and_eq_of_not_mem σ tt hnotmem with ⟨γ, heqod, hg⟩,
+        have : bodd (clause.count_tt γ (drop (k - 1) x ++ [Pos g.fresh.1])) = tt,
+        { simp only [count_tt_append, literal.eval, hg, cond, 
+            ← count_tt_eq_of_eqod (eqod_subset hdropvars heqod), he, bodd_succ,
+            bool.bnot_false, count_tt_singleton, bodd_succ] },
+        rw [← eval_eq_bodd_count_tt, ← eval_direct_xor_eq_eval_Xor] at this,
+
+        -- Apply the induction hypothesis
+        rcases (ih _ h₁ h₂ γ).mpr ⟨γ, this, eqod.refl _ _⟩ with ⟨γ₂, he₂, hg₂⟩,
+
+        have heqod₂ : eqod (assignment.ite (cnf.vars (pooled_xor hk (drop (k - 1) x ++ [Pos g.fresh.1]) g.fresh.2 h₂)) γ₂ γ) γ (clause.vars x),
+        { intros v hv,
+          by_cases hmem : v ∈ vars (x.drop (k - 1)),
+          { rw vars at hmem,
+            have h₃ : v ∈ vars (drop (k - 1) x ++ [Pos g.fresh.1]),
+            { rw [vars, clause.vars_append],
+              exact finset.mem_union_left _ hmem },
+            rw [ite_pos _ _ (mem_pooled_xor_vars_of_mem_vars hk h₂ h₃), hg₂ v h₃] },
+          { have hdis₂ := set.disjoint_right.mp hdis hv,
+            have hne : v ≠ g.fresh.1,
+            { intro hcon,
+              exact (hcon ▸ hdis₂) (fresh_mem_stock g) },
+            have : v ∉ vars (drop (k - 1) x ++ [Pos g.fresh.1]),
+            { simp [vars, clause.vars, var, clause.vars_append],
+              rintros (hcon | hcon),
+              { rw vars at hmem, exact hmem hcon },
+              { exact hne hcon } },
+            have hstock : v ∉ g.fresh.2.stock,
+            { intro hcon,
+              exact hdis₂ ((fresh_stock_subset g) hcon) },
+            rw ite_neg _ _ (not_mem_pooled_xor_vars_of_not_mem_vars_of_not_mem_stock hk h₂ this hstock) } },
+        
+        use assignment.ite (cnf.vars (pooled_xor hk (drop (k - 1) x ++ [Pos g.fresh.1]) g.fresh.2 h₂)) γ₂ γ,
+        split,
+        { split,
+          { simp [eval_direct_xor_eq_eval_Xor, eval_eq_bodd_count_tt, 
+              count_tt_append, bodd_add, literal.eval, hg],
+            have : g.fresh.1 ∈ vars (drop (k - 1) x ++ [Pos g.fresh.1]),
+            { simp [vars, clause.vars_append, var] },
+            simp [ite_pos _ _ (mem_pooled_xor_vars_of_mem_vars hk h₂ this), 
+              ← (hg₂ g.fresh.1 this), hg,
+              count_tt_eq_of_eqod (eqod_subset htakevars heqod₂),
+              ← count_tt_eq_of_eqod (eqod_subset htakevars heqod), hc] },
+          { exact he₂ ▸ eval_eq_cnf_of_eqod (ite_eqod _ _ _) } },
+        { exact eqod.trans (eqod.trans hs heqod) heqod₂.symm } } } }
 end
 
 end tseitin_xor
